theories/logrel/typing.v
@@ -117,8 +117,7 @@ Inductive has_type (Γ : stringmap type) :
     has_type Γ (e1 <- e2) tunit
 | CAS_typed e1 e2 e3 τ :
     unboxed_type τ →
-    flat_type τ →
-    has_type Γ e1 (tref (stamp τ (lbl τ))) →
+    has_type Γ e1 (tref τ) →
     has_type Γ e2 τ →
     has_type Γ e3 τ →
     has_type Γ (CAS e1 e2 e3) (tbool (lbl τ))
